switching to proper parallel beta

thys/Untyped_Lambda_Calculus/LC_Beta.thy
@@ -1,3 +1,5 @@
+(* Here we instantiate the general enhanced rule induction to parallel beta reduction
+for the (untyped) lambda-calculus *)
 theory LC_Beta 
 imports LC  "../Instantiation_Infrastructure/Curry_LFP" 
 "../Generic_Barendregt_Enhanced_Rule_Induction"
@@ -18,10 +20,10 @@ apply standard
 (* (a reduced form of) small step semantics *) 
 
 inductive step :: "trm \<Rightarrow> trm \<Rightarrow> bool" where
-  Beta: "step (App (Abs x e1) e2) (tvsubst (VVr(x:=e2)) e1)"
-| AppL: "step e1 e1' \<Longrightarrow> step (App e1 e2) (App e1' e2)"
+  Refl: "step e e"
+| App: "step e1 e1' \<Longrightarrow> step e2 e2' \<Longrightarrow> step (App e1 e2) (App e1' e2')"
 | Xi: "step e e' \<Longrightarrow> step (Abs x e) (Abs x e')"
-|PBeta: "step e1 e1' \<Longrightarrow> step e2 e2' \<Longrightarrow> step (App (Abs x e1) e2) (tvsubst (VVr(x:=e2')) e1')"
+| PBeta: "step e1 e1' \<Longrightarrow> step e2 e2' \<Longrightarrow> step (App (Abs x e1) e2) (tvsubst (Var(x:=e2')) e1')"
 
 thm step_def
 
@@ -55,13 +57,14 @@ apply standard unfolding ssbij_def Tmap_def Vmap_def
 definition G :: "(T \<Rightarrow> bool) \<Rightarrow> V \<Rightarrow> T \<Rightarrow> bool"
 where
 "G \<equiv> \<lambda>R v t.  
-         (\<exists>x e1 e2. v = [x] \<and> fst t = App (Abs x e1) e2 \<and> snd t = tvsubst (VVr(x := e2)) e1)
+         (v = [] \<and> fst t = snd t)
          \<or>
-         (\<exists>e1 e1' e2. v = [] \<and> fst t = App e1 e2 \<and> snd t = App e1' e2 \<and> R (e1,e1')) 
+         (\<exists>e1 e1' e2 e2'. v = [] \<and> fst t = App e1 e2 \<and> snd t = App e1' e2' \<and> 
+                           R (e1,e1') \<and> R (e2,e2')) 
          \<or>
          (\<exists>x e e'. v = [x] \<and> fst t = Abs x e \<and> snd t = Abs x e' \<and> R (e,e'))
          \<or>
-         (\<exists>x e1 e1' e2 e2'. v = [x] \<and> fst t = App (Abs x e1) e2 \<and> snd t = tvsubst (VVr(x := e2')) e1' \<and> 
+         (\<exists>x e1 e1' e2 e2'. v = [x] \<and> fst t = App (Abs x e1) e2 \<and> snd t = tvsubst (Var(x := e2')) e1' \<and> 
             R (e1,e1') \<and> R (e2,e2'))"
 
 
@@ -73,16 +76,14 @@ unfolding G_def by fastforce
 lemma GG_equiv: "ssbij \<sigma> \<Longrightarrow> G R v t \<Longrightarrow> G (\<lambda>t'. R (Tmap (inv \<sigma>) t')) (Vmap \<sigma> v) (Tmap \<sigma> t)"
 unfolding G_def apply(elim disjE)
   subgoal apply(rule disjI1)
-  subgoal apply(elim exE) subgoal for x e1 e2 
-  apply(rule exI[of _ "\<sigma> x"])
-  apply(rule exI[of _ "rrename_term \<sigma> e1"]) apply(rule exI[of _ "rrename_term \<sigma> e2"])
-  apply(cases t) unfolding ssbij_def small_def Tmap_def Vmap_def apply simp
-  apply(subst rrename_tvsubst_comp) by auto  . .
+  subgoal  
+  apply(cases t) unfolding ssbij_def small_def Tmap_def Vmap_def 
+  by simp . 
   (* *)
   subgoal apply(rule disjI2, rule disjI1)
-  subgoal apply(elim exE) subgoal for e1 e1' e2
+  subgoal apply(elim exE) subgoal for e1 e1' e2 e2'
   apply(rule exI[of _ "rrename_term \<sigma> e1"]) apply(rule exI[of _ "rrename_term \<sigma> e1'"]) 
-  apply(rule exI[of _ "rrename_term \<sigma> e2"])
+  apply(rule exI[of _ "rrename_term \<sigma> e2"]) apply(rule exI[of _ "rrename_term \<sigma> e2'"])
   apply(cases t) unfolding ssbij_def small_def Tmap_def Vmap_def 
   by (simp add: term.rrename_comps) . . 
   (* *)
@@ -110,19 +111,13 @@ lemma GG_fresh:
 "(\<forall>\<sigma> t. ssbij \<sigma> \<and> R t \<longrightarrow> R (Tmap \<sigma> t)) \<Longrightarrow> G R v t \<Longrightarrow> 
  \<exists>w. Vfvars w  \<inter> Tfvars t = {} \<and> G R w t"
 using fresh[of t] unfolding G_def Tmap_def Vmap_def apply safe
-  subgoal for xx x e1 e2
-  apply(rule exI[of _ "[xx]"])  
+  subgoal for xx
+  apply(rule exI[of _ "[]"])  
   apply(rule conjI)
     subgoal unfolding ssbij_def small_def Vmap_def by auto 
-    subgoal apply(rule disjI1) 
-    apply(rule exI[of _ "xx"]) 
-    apply(rule exI[of _ "rrename_term (id(x:=xx,xx:=x)) e1"])
-    apply(rule exI[of _ "e2"])
-    apply(cases t)  apply simp apply(intro conjI)
-      subgoal apply(subst Abs_rrename[of "id(x:=xx,xx:=x)"]) by auto
-      subgoal using tvsubst_Var_rrename_term by auto . .
+    subgoal apply(rule disjI1) by simp .
   (* *)
-  subgoal for xx e1 e1' e2
+  subgoal for xx e1 e1' e2 e2'
   apply(rule exI[of _ "[]"])  
   apply(rule conjI)
     subgoal unfolding ssbij_def small_def Vmap_def by auto 
@@ -130,6 +125,7 @@ using fresh[of t] unfolding G_def Tmap_def Vmap_def apply safe
     apply(rule exI[of _ "e1"]) 
     apply(rule exI[of _ "e1'"])
     apply(rule exI[of _ "e2"]) 
+    apply(rule exI[of _ "e2'"])
     apply(cases t)  apply simp . .
   (* *)
   subgoal for xx x e e'
@@ -172,27 +168,27 @@ apply standard
   using GG_mono GG_equiv GG_fresh by auto
 
 (* *)
-lemmas I_def = nitpick_unfold(178) 
 
 lemma step_I: "step t1 t2 = I (t1,t2)" 
   unfolding step_def I_def lfp_curry2 apply(rule arg_cong2[of _ _ _ _ lfp], simp_all)
-  unfolding fun_eq_iff G_def apply safe
-    subgoal apply simp by metis
+  unfolding fun_eq_iff G_def apply safe 
     subgoal by auto
-    subgoal by auto
-    subgoal apply simp by metis
     subgoal by auto
     subgoal by auto
     subgoal apply simp by metis
-    subgoal by auto .
+    subgoal by (metis fst_conv snd_conv)
+    subgoal by (metis fst_conv snd_conv)
+    subgoal by (metis fst_conv snd_conv)
+    subgoal by (metis fst_conv snd_conv) .
 
 (* FROM ABSTRACT BACK TO CONCRETE: *)
 thm step.induct[no_vars]
 
 corollary BE_induct_step: "(\<And>p. small (Pfvars p)) \<Longrightarrow> 
 step t1 t2 \<Longrightarrow> 
-(\<And>x e e2 p. x \<notin> Pfvars p \<Longrightarrow> x \<notin> FFVars_term e2 \<Longrightarrow> R p (App (Abs x e) e2) (tvsubst (VVr(x := e2)) e)) \<Longrightarrow>
-(\<And>e1 e1' e2 p. step e1 e1' \<Longrightarrow> (\<forall>p'. R p' e1 e1') \<Longrightarrow> R p (App e1 e2) (App e1' e2)) \<Longrightarrow> 
+(\<And>e p. R p e e) \<Longrightarrow>
+(\<And>e1 e1' e2 e2' p. step e1 e1' \<Longrightarrow> 
+  (\<forall>p'. R p' e1 e1') \<Longrightarrow> (\<forall>p'. R p' e2 e2') \<Longrightarrow> R p (App e1 e2) (App e1' e2')) \<Longrightarrow> 
 (\<And>e e' x p. x \<notin> Pfvars p \<Longrightarrow> step e e' \<Longrightarrow> (\<forall>p'. R p' e e') \<Longrightarrow> R p (Abs x e) (Abs x e')) \<Longrightarrow> 
 (\<And>x e e' e2 e2' p. x \<notin> Pfvars p \<Longrightarrow> step e e' \<Longrightarrow> (\<forall>p'. R p' e e') \<Longrightarrow> step e2 e2' \<Longrightarrow> (\<forall>p'. R p' e2 e2') \<Longrightarrow> 
    x \<notin> FFVars_term e2 \<Longrightarrow> (x \<in> FFVars_term e' \<Longrightarrow> x \<notin> FFVars_term e2') \<Longrightarrow> 
@@ -202,7 +198,7 @@ unfolding step_I
 apply(subgoal_tac "case (t1,t2) of (t1, t2) \<Rightarrow> R p t1 t2")
   subgoal by auto
   subgoal apply(erule BE_induct[where R = "\<lambda>p (t1,t2). R p t1 t2"])
-  unfolding G_def apply auto apply(subst (asm) FFVars_tvsubst) by (auto split: if_splits) .
+  unfolding G_def by (auto simp: FFVars_tvsubst split: if_splits) .
 
 
 end
